
\section{Verification \cite{Yan2013}, \cite{Paar2010}, \cite{Garrett2005}}
\setcounter{theorem}{0}
\setcounter{equation}{0}

%%%%%%%%%%%%%%%%%%%%%%%%%%%%%%%%%%%%%%%%

Receives the signed message
\,$\left(\,m \,\overset{{\color{white}.}}{;}\,(\,r,s\,)\,\right) \,\in\, \Sigma^{*} \times \Z_{q}^{*} \times \Z_{q}^{*}$.

\begin{itemize}
\item
	Retrieve the public verification key \,$A \,\in\, E$.
\item
	Compute \,$e \,=\, H(m) \,\in\, \{0,1,2,\ldots,N\}$.
\item
	Compute \,$u_{1} \,:=\, s^{-1} \cdot H(m) \!\mod q$.\; Note that \,$u_{1}\,\in\, \Z_{q}$.
\item
	Compute \,$u_{2} \,:=\, s^{-1} \cdot r \!\mod q$.\; Note that \,$u_{2}\,\in\, \Z_{q}$.
\item
	Compute \,$P \,=\, u_{1}\cdot G +  u_{2} \cdot A \,=\, (\,x_{P}\,,\, y_{P}\,) \,\in\, \Z_{p} \times \Z_{p}$
\end{itemize}

\noindent
Then,
\begin{center}
Accept signature\;\; if and only if \;\;$r \,=\, x_{P} \!\mod q$
\end{center}

%%%%%%%%%%%%%%%%%%%%%%%%%%%%%%%%%%%%%%%%

\vskip 0.8cm
\noindent
\textbf{Proof of validity of the ECDSA verification procdure}

\vskip 0.3cm
\noindent
More precisely, we prove that $x_{P} \in \Z_{p}$ indeed satisfies the equation:
\begin{equation*}
r \;=\; x_{P} \!\mod q
\end{equation*}
To this end, simply observe that
\begin{eqnarray*}
&&
	s \,:=\, k^{-1} \cdot\left(\,H(m) + a\,r\,\right) \!\mod q
\\
&\Longleftrightarrow&
	k \,=\, s^{-1} \cdot\left(\,H(m) + a\,r\,\right)	\!\mod q
\\
&\Longleftrightarrow&
	k \,=\, s^{-1} \cdot H(m) + a \cdot s^{-1} \cdot r \!\mod q
\\
&\Longleftrightarrow&
	k \,=\, u_{1} + a \cdot u_{2} \!\mod q
\\
&\Longrightarrow&
	R \,:=\, k \cdot G \,=\, \left(\,u_{1} + a \cdot u_{2} \,\right) \cdot G \,=:\, P \,\in\, E 
\\
&\Longrightarrow&
	r \;\;:=\;\; x_{R}\!\!\mod q \;\;=\;\; x_{P} \!\!\mod q
\end{eqnarray*}
\qed

%%%%%%%%%%%%%%%%%%%%%%%%%%%%%%%%%%%%%%%%
\vskip 0.0cm
\noindent
References: \cite{Yan2013}, \cite{Paar2010}, \cite{Garrett2005}
